Style updates

RegexCorrectness/NFA/Transition/Path/Basic.lean
@@ -2,68 +2,66 @@ import RegexCorrectness.NFA.Basic
 
 namespace Regex.NFA
 
-inductive stepIn (nfa : NFA) (start : Nat) : (current next : Nat) → (cs : List Char) → Prop where
-  | charStep {i j : Nat} {c : Char} (h₁ : start ≤ i) (h₂ : i < nfa.nodes.size) (step : j ∈ nfa[i].charStep c) : nfa.stepIn start i j [c]
-  | εStep {i j : Nat} (h₁ : start ≤ i) (h₂ : i < nfa.nodes.size) (step : j ∈ nfa[i].εStep) : nfa.stepIn start i j []
+inductive stepIn (nfa : NFA) (lowerBound : Nat) : (current next : Nat) → (cs : List Char) → Prop where
+  | charStep {i j : Nat} {c : Char} (h₁ : lowerBound ≤ i) (h₂ : i < nfa.nodes.size) (step : j ∈ nfa[i].charStep c) : nfa.stepIn lowerBound i j [c]
+  | εStep {i j : Nat} (h₁ : lowerBound ≤ i) (h₂ : i < nfa.nodes.size) (step : j ∈ nfa[i].εStep) : nfa.stepIn lowerBound i j []
 
-theorem stepIn.h₁ {nfa : NFA} {start : Nat} {i j : Nat} {cs : List Char}
-  (step : nfa.stepIn start i j cs) : start ≤ i := by
+theorem stepIn.h₁ {nfa : NFA} {lb i j : Nat} {cs : List Char}
+  (step : nfa.stepIn lb i j cs) : lb ≤ i := by
   cases step with
   | charStep h₁ _ _ => exact h₁
   | εStep h₁ _ _ => exact h₁
 
-theorem stepIn.h₂ {nfa : NFA} {start : Nat} {i j : Nat} {cs : List Char}
-  (step : nfa.stepIn start i j cs) : i < nfa.nodes.size := by
+theorem stepIn.h₂ {nfa : NFA} {lb i j : Nat} {cs : List Char}
+  (step : nfa.stepIn lb i j cs) : i < nfa.nodes.size := by
   cases step with
   | charStep _ h₂ _ => exact h₂
   | εStep _ h₂ _ => exact h₂
 
-theorem stepIn.step {nfa : NFA} {start : Nat} {i j : Nat} {cs : List Char}
-  (step : nfa.stepIn start i j cs) :
+theorem stepIn.step {nfa : NFA} {lb i j : Nat} {cs : List Char}
+  (step : nfa.stepIn lb i j cs) :
   (∃ c, j ∈ (nfa[i]'step.h₂).charStep c) ∨ j ∈ (nfa[i]'step.h₂).εStep := by
   cases step with
   | charStep _ _ step => exact .inl ⟨_, step⟩
   | εStep _ _ step => exact .inr step
 
-theorem le_of_stepIn {start} (step : stepIn nfa start i j cs) : start ≤ i := by
+theorem le_of_stepIn (step : stepIn nfa lb i j cs) : lb ≤ i := by
   cases step with
   | charStep h₁ => exact h₁
   | εStep h₁ => exact h₁
 
-theorem stepIn.lt_right {start} (step : stepIn nfa start i j cs) : j < nfa.nodes.size := by
+theorem stepIn.lt_right (step : stepIn nfa lb i j cs) : j < nfa.nodes.size := by
   match step.step with
   | .inl ⟨_, step⟩ => exact lt_of_charStep step
   | .inr step => exact lt_of_εStep step
 
-theorem stepIn.castStart' {nfa : NFA} {start start' : Nat}
-  (le : start' ≤ i) (step : stepIn nfa start i j cs) :
-  nfa.stepIn start' i j cs := by
+theorem stepIn.castBound' {nfa : NFA} (le : lb' ≤ i) (step : stepIn nfa lb i j cs) :
+  nfa.stepIn lb' i j cs := by
   cases step with
   | charStep h₁ h₂ step => exact .charStep le h₂ step
   | εStep h₁ h₂ step => exact .εStep le h₂ step
 
-theorem stepIn.castStart {nfa : NFA} {start start' : Nat}
-  (le : start' ≤ start) (step : stepIn nfa start i j cs) :
-  nfa.stepIn start' i j cs := step.castStart' (Nat.le_trans le step.h₁)
+theorem stepIn.castBound {nfa : NFA} (le : lb' ≤ lb) (step : stepIn nfa lb i j cs) :
+  nfa.stepIn lb' i j cs := step.castBound' (Nat.le_trans le step.h₁)
 
-theorem stepIn.cast {nfa nfa' : NFA} {start : Nat}
-  (step : nfa.stepIn start i j cs)
+theorem stepIn.cast {nfa nfa' : NFA}
+  (step : nfa.stepIn lb i j cs)
   (h : i < nfa'.nodes.size)
   (eq : nfa[i]'(step.h₂) = nfa'[i]) :
-  nfa'.stepIn start i j cs := by
+  nfa'.stepIn lb i j cs := by
   cases step with
   | charStep h₁ h₂ step =>
     exact .charStep h₁ h (eq ▸ step)
   | εStep h₁ h₂ step =>
     exact .εStep h₁ h (eq ▸ step)
 
-theorem stepIn.nil_or_singleton {start} (h : stepIn nfa start i j cs) :
+theorem stepIn.nil_or_singleton (h : stepIn nfa lb i j cs) :
   cs = [] ∨ ∃ c, cs = [c] := by
   cases h with
   | εStep => exact .inl rfl
   | charStep => exact .inr ⟨_, rfl⟩
 
-theorem stepIn.nil_of_snoc {start} (h : stepIn nfa start i j (cs ++ [c])) :
+theorem stepIn.nil_of_snoc (h : stepIn nfa lb i j (cs ++ [c])) :
   cs = [] := by
   generalize h' : cs ++ [c] = cs' at h
   cases h with
@@ -75,8 +73,17 @@ theorem stepIn.nil_of_snoc {start} (h : stepIn nfa start i j (cs ++ [c])) :
       have := congrArg List.length h'
       simp at this
 
--- Idea: what if we require at least one step? (Making this a non-reflexive transitive closure)
--- TODO: expand the motivation
+/--
+
+A predicate that represents a path in a NFA, with each starting node being at least `lowerBound`.
+
+## Motivation
+
+When we reason about an NFA constructed by `pushRegex nfa next r`, we are typically intersted in
+paths that uses only the nodes added by `pushRegex` (and the last step to escape to `next`).
+The definition of `pathIn` limits `first` to be at least `lowerBound` to capture this notion.
+
+-/
 inductive pathIn (nfa : NFA) (lowerBound : Nat) : (first : Nat) → (last : Nat) → (cs : List Char) → Prop where
   | last (step : nfa.stepIn lowerBound i j cs) : nfa.pathIn lowerBound i j cs
   | more {i j k : Nat} {cs₁ cs₂ : List Char}
@@ -102,8 +109,8 @@ theorem pathIn.castBound {nfa : NFA} {lb lb' : Nat}
   (path : nfa.pathIn lb i j cs) :
   nfa.pathIn lb' i j cs := by
   induction path with
-  | last step => exact .last (step.castStart le)
-  | more step _ ih => exact .more (step.castStart le) ih
+  | last step => exact .last (step.castBound le)
+  | more step _ ih => exact .more (step.castBound le) ih
 
 theorem pathIn.cast {nfa nfa' : NFA} (lb : Nat)
   (eq : ∀ i, (h₁ : lb ≤ i) → (h₂ : i < nfa.nodes.size) → ∃ h' : i < nfa'.nodes.size, nfa[i] = nfa'[i])
@@ -139,9 +146,9 @@ theorem pathIn.castLE {nfa : NFA} {lb lb' i i' : Nat}
   (path : pathIn nfa lb i i' cs) :
   pathIn nfa lb' i i' cs := by
   induction path with
-  | last step => exact .last (step.castStart' assm)
+  | last step => exact .last (step.castBound' assm)
   | @more i j k cs₁ cs₂ step rest ih =>
-    have step' := step.castStart' assm
+    have step' := step.castBound' assm
     have : lb' ≤ j := by
       cases step with
       | charStep _ h₂ step => exact inBounds i j assm h₂ (.inl ⟨_, step⟩) rest.le_left
@@ -155,10 +162,10 @@ theorem pathIn.snoc_char (path : pathIn nfa lb i j cs) (assm : min lb k ≤ j)
   induction path with
   | @last i j cs step' =>
     have step'' : nfa.stepIn (min lb k) j k [c] := .charStep assm step'.lt_right step
-    exact .more (step'.castStart (Nat.min_le_left lb k)) (.last step'')
+    exact .more (step'.castBound (Nat.min_le_left lb k)) (.last step'')
   | @more i j k cs₁ cs₂ step' _ ih =>
     simp
-    exact .more (step'.castStart (Nat.min_le_left _ _)) (ih assm step)
+    exact .more (step'.castBound (Nat.min_le_left _ _)) (ih assm step)
 
 theorem pathIn.snoc_ε (path : pathIn nfa lb i j cs) (assm : min lb k ≤ j)
   (step : k ∈ (nfa[j]'path.lt_right).εStep)
@@ -169,9 +176,9 @@ theorem pathIn.snoc_ε (path : pathIn nfa lb i j cs) (assm : min lb k ≤ j)
       simp at this
       exact this
     have step'' : nfa.stepIn (min lb k) j k [] := .εStep assm step'.lt_right step
-    exact .more (step'.castStart (Nat.min_le_left lb k)) (.last step'')
+    exact .more (step'.castBound (Nat.min_le_left lb k)) (.last step'')
   | @more i j k cs₁ cs₂ step' _ ih =>
-    exact .more (step'.castStart (Nat.min_le_left _ _)) (ih assm step)
+    exact .more (step'.castBound (Nat.min_le_left _ _)) (ih assm step)
 
 theorem pathIn.trans (path₁ : pathIn nfa lb i j cs) (path₂ : pathIn nfa lb j k cs') :
   pathIn nfa lb i k (cs ++ cs') := by
